src/sf_proof.v
@@ -52,21 +52,27 @@ Qed.
 
 Lemma eliminated_correct :
 forall rec can,
-sf_imp.eliminated candidate _ rec can = true ->
+sf_imp.eliminated candidate _ rec can = true <->
 in_record rec can.
 Proof.
+split.
 intros.
 unfold sf_imp.eliminated in *. rewrite existsb_exists in H.
 destruct H; intuition.
 rewrite existsb_exists in H1. destruct H1; intuition.
 unfold in_record.
 apply reldec_correct_candidate in H2. subst; eauto.
+intros.
+unfold sf_imp.eliminated in *. rewrite existsb_exists.
+unfold in_record in H. destruct H. exists x. intuition.
+rewrite existsb_exists. exists can. intuition.
+apply reldec_correct_candidate. auto.
 Qed.
 
 Definition no_viable_candidates eliminated (b : sf_spec.ballot candidate) :=
 Forall (Forall eliminated) b.
 
-Lemma no_viable_candidate_Forall :
+Lemma no_viable_candidates_Forall :
 forall eliminated b,
 no_viable_candidates eliminated b <->
 sf_spec.no_viable_candidates candidate eliminated b.
@@ -82,30 +88,36 @@ specialize (H x). intuition.
 Qed.
 
 Lemma next_ranking_correct :
-forall rec bal cd bal',
+forall rec bal cd bal' ,
 sf_imp.next_ranking candidate _ rec bal = Some (cd, bal') ->
-sf_spec.next_ranking candidate (in_record rec) bal [cd].
+exists l,(sf_spec.next_ranking candidate (in_record rec) bal l /\ Forall (eq cd) l).
 Proof.
 intros.
 induction bal.
 - simpl in *. congruence.
 - simpl in *.
   destruct a.
-  + intuition.
-  + destruct a.
+  + intuition. destruct H0. exists x. intuition.
+  + destruct (forallb (eq_dec c) a) eqn:Heqb0.
     * { destruct (sf_imp.eliminated candidate reldec_candidate rec c) eqn:?.
-         - apply IHbal in H.
-           left. split. 
-           + intros. inversion H0. 
-             * subst.
-               unfold sf_imp.eliminated in Heqb. rewrite existsb_exists in Heqb.
-               destruct Heqb. intuition. rewrite existsb_exists in H3. destruct H3.
-               destruct H1.  apply reldec_correct_candidate in H3. subst.
-               unfold in_record. exists x. auto.
-             * inversion H1.
-           + auto.
-         - inversion H. subst. clear H.
-           right.
+         - apply IHbal in H. clear IHbal.
+           destruct H. destruct H. exists x.
+           split. left. intuition.
+           + intros.
+             assert (c = c0).
+             destruct H1. auto.
+             rewrite forallb_forall in Heqb0.
+             apply Heqb0 in H1.
+             apply reldec_correct_candidate in H1. auto.
+             subst.
+             unfold sf_imp.eliminated in Heqb. rewrite existsb_exists in Heqb.
+             destruct Heqb. intuition. rewrite existsb_exists in *. destruct H4.
+             destruct H2. apply reldec_correct_candidate in H4. subst.
+             unfold in_record. eauto.               
+           + intuition.
+         - inversion H. subst. clear H. 
+           exists (cd :: a).
+           split. right.
            split.
            + unfold sf_imp.eliminated in *. 
              apply existsb_false_forall in Heqb.
@@ -125,12 +137,152 @@ induction bal.
                unfold eq_dec in *.
                congruence.
            + reflexivity.
+           + rewrite forallb_forall in Heqb0. rewrite Forall_forall. 
+             intuition. destruct H. auto. apply Heqb0 in H. apply reldec_correct_candidate.
+             auto.                                                                     
       } 
-    * congruence.
+    * congruence.       
 Qed.
 
 
+Lemma next_ranking_in :
+forall e bal x,
+  sf_spec.next_ranking candidate e bal x ->
+  In x bal.
+Proof.
+induction bal; intros.
+- simpl in H. auto.
+- simpl in *. intuition.
+Qed.
 
+Lemma next_ranking_cons_or :
+forall b1 bal e x,
+sf_spec.next_ranking candidate e (b1 :: bal) x ->
+sf_spec.next_ranking candidate e [b1] x \/ 
+sf_spec.next_ranking candidate e bal x.
+intros. simpl in  H. intuition. destruct H. destruct H.
+left. unfold sf_spec.next_ranking. right. eauto.
+Qed.
+
+Ltac inv H := inversion H; subst; clear H.
+
+Lemma overvote_cons_or :
+forall b1 bal e ,
+sf_spec.overvote candidate e (b1 :: bal) ->
+sf_spec.overvote candidate e [b1] \/ sf_spec.overvote candidate e bal.
+Proof.
+intros.
+inv H.  
+intuition.
+destruct H1. destruct H0.
+intuition.
+edestruct (next_ranking_cons_or); eauto.
+- unfold sf_spec.overvote.
+  left. exists x. split; eauto.
+- right. unfold sf_spec.overvote. exists x; split; eauto.
+Qed.
+
+Lemma next_ranking_not_overvote :
+forall rec bal cd bal',
+sf_imp.next_ranking candidate _ rec bal = Some (cd, bal') ->
+~sf_spec.overvote candidate (in_record rec) bal.
+Proof.
+intros.
+induction bal.
+- simpl in *. congruence.
+- simpl in *.
+  destruct a.
+  + intro.
+    unfold sf_spec.overvote in H0.
+    destruct H0.
+    destruct H0.
+    simpl in H0.
+    intuition. 
+    unfold sf_spec.overvote in H2. apply H2. eauto.
+    subst. destruct H1. destruct H1. intuition.
+  + destruct (forallb (eq_dec c) a) eqn:?.
+    * { destruct (sf_imp.eliminated candidate reldec_candidate rec c) eqn:?.
+        - intuition. 
+          edestruct (overvote_cons_or); eauto.
+          + rewrite forallb_forall in *. 
+            clear -H2 Heqb reldec_correct_candidate.
+            inversion H2. intuition.
+            inversion H0. intuition.
+            intuition. subst. intuition.
+            destruct H1. destruct H.
+            intuition. apply H5.
+            simpl in *. intuition; subst; auto. 
+            * specialize (Heqb x0). intuition.
+              apply reldec_correct_candidate in H. auto.
+            * specialize (Heqb x). intuition.
+              apply reldec_correct_candidate in H. auto.
+            * assert (x = c).
+              specialize (Heqb x). intuition. apply reldec_correct_candidate in H.
+              auto.
+              assert (x0 = c).               
+              specialize (Heqb x0). intuition. apply reldec_correct_candidate in H7.
+              auto.
+              subst. auto.
+        - inv H. intro.
+          inv H. clear IHbal.
+          intuition.
+          destruct H1. destruct H0. intuition. inv H.
+          destruct H2. specialize (H cd). simpl in H. intuition.
+          rewrite <- eliminated_correct in H. congruence.
+          intuition. subst.
+          apply H3.
+          rewrite forallb_forall in Heqb. 
+          simpl in *. intuition; subst; auto.
+          + specialize (Heqb _ H1). apply reldec_correct_candidate in Heqb. 
+            auto.
+          + specialize (Heqb _ H2). apply reldec_correct_candidate in Heqb.
+            auto.
+          + assert (x0 = cd); subst. 
+            specialize (Heqb _ H2). apply reldec_correct_candidate in Heqb. auto.
+            assert (x1 = cd); subst.
+            specialize (Heqb _ H1). apply reldec_correct_candidate in Heqb. auto.
+            auto. } 
+    * congruence.
+Qed.
+    
+Lemma no_viable_candidates_cons :
+forall a b e,
+sf_spec.no_viable_candidates candidate (e) (a ::  b) ->
+sf_spec.no_viable_candidates candidate e [a] /\
+sf_spec.no_viable_candidates candidate e b.
+intros.
+unfold sf_spec.no_viable_candidates in *.
+split.
+intros. eapply H; eauto. inv H0; simpl in *; intuition.
+intros. eapply H; eauto. simpl. intuition.
+Qed.
+
+Lemma next_ranking_viable :
+forall bal rec cd bal',
+sf_imp.next_ranking candidate reldec_candidate rec bal =
+      Some (cd, bal') ->
+~sf_spec.no_viable_candidates candidate (in_record rec) bal.
+Proof.
+induction bal; intros.
+- simpl in *. congruence.
+- simpl in *. destruct a.
+  + intro. apply no_viable_candidates_cons in H0. destruct H0.
+    eapply IHbal in H1; eauto.
+  + destruct (forallb (eq_dec c) a).
+    * { destruct (sf_imp.eliminated candidate reldec_candidate rec c) eqn:?.
+        - apply eliminated_correct in Heqb.
+          intro. apply no_viable_candidates_cons in H0.
+          destruct H0.
+          eapply IHbal in H1; eauto.
+        - inv H. intro. apply no_viable_candidates_cons in H. destruct H.
+          unfold sf_spec.no_viable_candidates in H. 
+          specialize (H (cd :: a)). simpl in H. intuition. clear H2.
+          specialize (H cd). intuition. clear H2. 
+          rewrite <- eliminated_correct in H. congruence.
+      }
+    * congruence.
+Qed.
+  
 
 Lemma next_ranking_selected :
 forall bal cd bal' rec,
@@ -138,42 +290,19 @@ sf_imp.next_ranking candidate _ rec bal = Some (cd, bal') ->
 sf_spec.selected_candidate candidate (in_record rec) bal cd.
 intros.
 unfold sf_spec.selected_candidate. split.
-unfold sf_spec.continuing_ballot. intro.
-induction bal.
-- simpl in *. congruence.
-- simpl in *.
-  destruct a.
-  + intuition. unfold sf_spec.exhausted_ballot in H0.
-    destruct H0.
-    * unfold sf_spec.exhausted_ballot in H1.
-      apply H1.
-      left.
-      unfold sf_spec.no_viable_candidates in H0.
-      intro. intros.
-      eapply H0; eauto. simpl. right. auto.
-    * apply H1. unfold sf_spec.exhausted_ballot.
-      right.
-      unfold sf_spec.overvote in *.
-      destruct H0. exists x. intuition.
-      simpl in H2. intuition. 
-      destruct H2. intuition.
-  + destruct a.
-    destruct ( sf_imp.eliminated candidate reldec_candidate rec c) eqn:?.
-    intuition.
-    apply H1. apply eliminated_correct in Heqb.
-    unfold sf_spec.exhausted_ballot in H0. destruct H0.
-    rewrite  <- no_viable_candidate_Forall in H0.
-    unfold no_viable_candidates in H0.
-    inversion H0. subst.
-    unfold sf_spec.exhausted_ballot.
-    rewrite <- no_viable_candidate_Forall. intuition.
-Admitted.    
+- unfold sf_spec.continuing_ballot. intro. 
+  unfold sf_spec.exhausted_ballot in H0.
+  destruct H0. 
+  + apply next_ranking_viable in H. auto.
+  + eapply next_ranking_not_overvote in H0; eauto.
+- apply next_ranking_correct in H. destruct H. destruct H.
+  exists x. intuition.
+  destruct x. induction bal. inv H. simpl in *. intuition. subst. 
+  destruct H; intuition.
+  inv H0. simpl in *. auto.
+Qed.
 
-    
-
-
-
-   
+  
     
 
 Lemma tabulate_continuing :
